back to self-testing with TLS 1.2

src/tls/test/TestAPI.fst
@@ -11,27 +11,39 @@ open TLS
 
 module CC = CoreCrypto
 
+inline_for_extraction let api_debug = true
+val discard: bool -> ST unit
+  (requires (fun _ -> True))
+  (ensures (fun h0 _ h1 -> h0 == h1))
+let discard _ = ()
+let print s = discard (IO.debug_print_string ("API| "^s^"\n"))
+unfold val trace: s:string -> ST unit
+  (requires (fun _ -> True))
+  (ensures (fun h0 _ h1 -> h0 == h1))
+unfold let trace = if api_debug then print else (fun _ -> ())
+
+
 let rec read_loop con r : ML unit =
   match TLS.read con r with
   | Read (DataStream.Data d) ->
     let db = DataStream.appBytes d in
-    IO.print_string ("Received data: "^(iutf8 db));
+    trace ("Received data: "^(iutf8 db));
     read_loop con r
   | ReadError _ t ->
-    IO.print_string ("ReadError: "^t^"\n")
+    trace ("ReadError: "^t^"\n")
   | Read (DataStream.Close) ->
-    IO.print_string "Got close_notify, closing connection...\n";
+    trace "Got close_notify, closing connection...\n";
     let _ = TLS.writeCloseNotify con in
     ()
   | Read (DataStream.Alert a)->
-    IO.print_string ("Got alert: "^(string_of_ad a)^"\n");
-    IO.print_string "Closing connection.\n";
+    trace ("Got alert: "^(string_of_ad a)^"\n");
+    trace "Closing connection.\n";
     let _ = TLS.writeCloseNotify con in
     ()
 
 private
 let client config host port =
-  IO.print_string "===============================================\n Starting test TLS client...\n";
+  trace "*** Starting test TLS client...";
   let tcp = Transport.connect host port in
   let rid = new_region root in
   let con = TLS.connect rid tcp config in
@@ -39,7 +51,7 @@ let client config host port =
   let id = TLS.currentId con Reader in
   match TLS.read con id with
     | Complete ->
-       IO.print_string "Read OK, sending HTTP request...\n";
+       trace "Read OK, sending HTTP request...";
        let payload = utf8 ("GET /r HTTP/1.1\r\nConnection: close\r\nHost: " ^ host ^ "\r\n\r\n") in
        let id = TLS.currentId con Writer in
        let rg : Range.frange id = Range.point (length payload) in
@@ -48,26 +60,30 @@ let client config host port =
        | Written ->
          let r = TLS.currentId con Reader in
          read_loop con r
-       | WriteError _ t -> IO.print_string ("Write error:"^t^"\n")
-       | _ -> IO.print_string "unexpted ioresult_w\n")
+       | WriteError _ t -> trace ("Write error:"^t)
+       | _ -> trace "unexpected ioresult_w")
     | ReadError o t ->
-      IO.print_string ("ReadError: "^t^"\n")
-    | _ -> IO.print_string "unexpected ioresult_i read\n"
+      trace ("ReadError: "^t)
+    | _ -> trace "unexpected ioresult_i read"
 
 private let rec aux_server config sock : ML unit =
   let rid = new_region root in
   let con = TLS.accept rid sock config in
   let id = TLS.currentId con Reader in
 
-  let () = match TLS.read con id with
+  let r = TLS.read con id in 
+  trace (TLS.string_of_ioresult_i r); 
+  let () = match r with
   | Complete ->
    begin
     let id = TLS.currentId con Reader in
-    match TLS.read con id with
+    let r = TLS.read con id in
+    trace (TLS.string_of_ioresult_i r); 
+    match r with
     | Read (DataStream.Data d) ->
      begin
       let db = DataStream.appBytes d in
-      IO.print_string ("Received data: "^(iutf8 db));
+      trace ("Received data: "^(iutf8 db));
       let text = "You are connected to miTLS*!\r\n"
         ^ "This is the request you sent:\r\n\r\n" ^ (iutf8 db) in
       let payload = utf8 ("HTTP/1.1 200 OK\r\nConnection: close\r\nContent-Length:"
@@ -79,20 +95,21 @@ private let rec aux_server config sock : ML unit =
       match TLS.write con f with
       | Written  ->
        begin
-        IO.print_string "Reading again\n";
+        trace "Reading again\n";
         let id = TLS.currentId con Reader in
         match TLS.read con id with
-        | Read DataStream.Close -> IO.print_string "Received close_notify! Closing socket.\n"
-        | _ -> IO.print_string "improperly closed connection\n"
+        | Read DataStream.Close -> trace "Received close_notify! Closing socket."
+        | _ -> trace "improperly closed connection."
        end
-      | _ -> IO.print_string "failed to write HTTP response\n"
+      | _ -> trace "failed to write HTTP response."
      end
-    | _ -> IO.print_string "unexpected ioresult_w\n"
+    | Read (DataStream.Alert a) -> trace ("unexpected alert: "^string_of_ad a)
+    | _ -> trace "unexpected read result"
    end
-  | _ -> IO.print_string "unexpected ioresult_i read\n"
+  | _ -> trace "unexpected ioresult_i read."
   in aux_server config sock
 
 let server config host port =
- IO.print_string "===============================================\n Starting test TLS server...\n";
+ trace "*** Starting test TLS server ***";
  let sock = Platform.Tcp.listen host port in
  aux_server config sock
